theories/lang/cpp/logic/builtins.v
@@ -66,15 +66,14 @@ Section wp_builtin.
   Proof. intros. iIntros "[]". Qed.
 
   Axiom wp_expect : forall exp c Q,
-      Q exp |-- wp_builtin Bin_expect (Tfunction Ti64 (Ti64 :: Ti64 :: nil)) (exp :: c :: nil) Q.
+      Q exp |-- wp_builtin Bin_expect (Tfunction Tlong (Tlong :: Tlong :: nil)) (exp :: c :: nil) Q.
 
   (** Bit computations
    *)
-
   (* Returns one plus the index of the least significant 1-bit of x,
      or if x is zero, returns zero. *)
-  Definition ffs_spec (sz : bitsize) (n : Z) (Q : val -> epred) : mpred :=
-    [| has_type_prop (Vint n) (Tnum sz Signed) |] ** Q (Vint (first_set sz n)).
+  Definition ffs_spec sz (n : Z) (Q : val -> epred) : mpred :=
+    [| has_type_prop (Vint n) (Tnum sz Signed) |] ** Q (Vint (first_set (int_type.bitsN sz) n)).
 
   Axiom wp_ffs : forall sz c Q,
           ffs_spec sz c Q
@@ -92,8 +91,8 @@ Section wp_builtin.
      significant bit position. If x is 0, the result is undefined. *)
 
 
-  Definition ctz_spec (sz : bitsize) (n : Z) (Q : val -> epred) : mpred :=
-    [| has_type_prop (Vint n) (Tnum sz Unsigned) |] ** [| n <> 0 |] ** Q (Vint (trailing_zeros sz n)).
+  Definition ctz_spec sz (n : Z) (Q : val -> epred) : mpred :=
+    [| has_type_prop (Vint n) (Tnum sz Unsigned) |] ** [| n <> 0 |] ** Q (Vint (trailing_zeros (int_type.bitsN sz) n)).
 
   Axiom wp_ctz : forall sz c Q,
           ctz_spec sz c Q
@@ -109,8 +108,8 @@ Section wp_builtin.
 
   (* Returns the number of leading 0-bits in x, starting at the most significant
      bit position. If x is 0, the result is undefined. *)
-  Definition clz_spec (sz : bitsize) (n : Z) (Q : val -> epred) : mpred :=
-    [| has_type_prop (Vint n) (Tnum sz Unsigned) |] ** [| n <> 0 |] ** Q (Vint (leading_zeros sz n)).
+  Definition clz_spec sz (n : Z) (Q : val -> epred) : mpred :=
+    [| has_type_prop (Vint n) (Tnum sz Unsigned) |] ** [| n <> 0 |] ** Q (Vint (leading_zeros (int_type.bitsN sz) n)).
 
   Axiom wp_clz : forall sz c Q,
           clz_spec sz c Q
@@ -127,22 +126,22 @@ Section wp_builtin.
   (* Returns x with the order of the bytes reversed; for example, 0xaabb becomes
      0xbbaa. Byte here always means exactly 8 bits. *)
   Axiom wp_bswap16 : forall x Q,
-          [| has_type_prop (Vint x) Tu16 |] ** Q (Vint (bswap W16 x))
-      |-- wp_builtin Bin_bswap16 (Tfunction Tu16 (Tu16 :: nil))
+          [| has_type_prop (Vint x) Tushort |] ** Q (Vint (bswap bitsize.W16 x))
+      |-- wp_builtin Bin_bswap16 (Tfunction Tushort (Tushort :: nil))
           (Vint x :: nil) Q.
 
   Axiom wp_bswap32 : forall x Q,
-          [| has_type_prop (Vint x) Tu32 |] ** Q (Vint (bswap W32 x))
-      |-- wp_builtin Bin_bswap32 (Tfunction Tu32 (Tu32 :: nil))
+          [| has_type_prop (Vint x) Tuint |] ** Q (Vint (bswap bitsize.W32 x))
+      |-- wp_builtin Bin_bswap32 (Tfunction Tuint (Tuint :: nil))
           (Vint x :: nil) Q.
 
   Axiom wp_bswap64 : forall x Q,
-          [| has_type_prop (Vint x) Tu64 |] ** Q (Vint (bswap W64 x))
-      |-- wp_builtin Bin_bswap64 (Tfunction Tu64 (Tu64 :: nil))
+          [| has_type_prop (Vint x) Tulonglong |] ** Q (Vint (bswap bitsize.W64 x))
+      |-- wp_builtin Bin_bswap64 (Tfunction Tulonglong (Tulonglong :: nil))
           (Vint x :: nil) Q.
 
   Axiom wp_bswap128 : forall x Q,
-          [| has_type_prop (Vint x) Tu128 |] ** Q (Vint (bswap W128 x))
+          [| has_type_prop (Vint x) Tu128 |] ** Q (Vint (bswap bitsize.W128 x))
       |-- wp_builtin Bin_bswap128 (Tfunction Tu128 (Tu128 :: nil))
           (Vint x :: nil) Q.
 
