theories/lang/prelude/platform.v
@@ -14,7 +14,7 @@ Proof. solve_decision. Defined.
 (** ** bitsizes -- TODO represent simply as positive? *)
 Module bitsize.
   Variant t : Set :=
-    | W8 | W16 | W32 | W64 | W80 | W128.
+    | W8 | W16 | W32 | W64 (* | W80 *) | W128.
 
   Definition bitsN (b : t) : N :=
     match b with
@@ -22,11 +22,12 @@ Module bitsize.
     | W16 => 16
     | W32 => 32
     | W64 => 64
-    | W80 => 80
+(*    | W80 => 80 *)
     | W128 => 128
     end.
 
   Notation bitsZ b := (Z.of_N (bitsN b)).
+  Notation bitsNat b := (N.to_nat (bitsN b)).
 
   #[global] Instance t_eq_dec: EqDecision t.
   Proof. solve_decision. Defined.
@@ -39,7 +40,7 @@ Module bitsize.
                | W16 => 2
                | W32 => 3
                | W64 => 4
-               | W80 => 5
+(*               | W80 => 5 *)
                | W128 => 6
                end)
              (λ b,
@@ -48,7 +49,7 @@ Module bitsize.
                | 2 => W16
                | 3 => W32
                | 4 => W64
-               | 5 => W80
+(*               | 5 => W80 *)
                | 6 => W128
                | _ => W8
                end)).
@@ -61,9 +62,12 @@ Module bitsize.
     | W16 => 2
     | W32 => 4
     | W64 => 8
-    | W80 => 10
+(*    | W80 => 10 *)
     | W128 => 16
     end.
+
+  Notation byteZ b := (Z.of_N (bytesN b)).
+  Notation bytesNat b := (N.to_nat (bytesN b)).
 
   Lemma bytes_bits b : (8 * bytesN b = bitsN b)%N.
   Proof. by destruct b. Qed.
